src/AtomicSteps.v
@@ -1,0 +1,100 @@
+Require Import Bool List String Peano_dec.
+Require Import Common FMap Syntax Semantics StepDet Serial.
+Require Import TrsSim.
+
+Definition StateTCond := StateT -> Prop.
+Definition TrsHelperCond := TrsHelper -> Prop.
+
+Definition OstCond := (StateTCond * TrsHelperCond)%type.
+Definition OssCond := M.t OstCond.
+Definition MsgValCond := Value -> ObjectStates -> Prop.
+Definition StepCond := (OssCond * MsgValCond)%type.
+
+Definition stepCondTop: StepCond := (M.empty _, fun _ _ => True).
+
+Definition updateOstCond (oidx: IdxT) (ostc: OstCond) (stc: StepCond): StepCond :=
+  ((fst stc)+[oidx <- ostc], snd stc).
+
+Definition OstCondHolds (ostc: OstCond) (ost: OState) :=
+  (fst ostc) (ost_st ost) /\ (snd ostc) (ost_tst ost).
+  
+Definition OssCondHolds (ossc: OssCond) (oss: ObjectStates) :=
+  (forall oidx,
+      match ossc@[oidx] with
+      | Some ostc => oss@[oidx] >>=[False] (fun ost => OstCondHolds ostc ost)
+      | None => True
+      end).
+
+Definition MsgValCondHolds (mvc: MsgValCond) (mval: Value) (oss: ObjectStates) :=
+  mvc mval oss.
+
+Definition StepCondHolds (stc: StepCond) (mval: Value) (oss: ObjectStates) :=
+  OssCondHolds (fst stc) oss /\ MsgValCondHolds (snd stc) mval oss.
+
+Section AtomicSteps.
+
+  Variables (trsIdx: IdxT)
+            (rqImpl rqSpec: Msg).
+
+  Variable (spec: System) (sobj: Object) (spmsg: PMsg)
+           (Hsobj: sys_objs spec = sobj :: nil)
+           (HspmsgIn: In spmsg (obj_trs sobj))
+           (Hspmsg: pmsg_mid spmsg = msg_id rqSpec).
+
+  Variables (impl: System)
+            (R: ObjectStates -> ObjectStates -> Prop)
+            (p: Label -> Label)
+            (HrqP: p (LblIn rqImpl) = LblIn rqSpec).
+  
+  Local Infix "≈" := R (at level 30).
+
+  Inductive AtomicSteps:
+    StepCond (* impl precondition *) ->
+    ObjectStates (* impl state *) ->
+    ObjectStates (* spec state *) ->
+    list Msg (* output messages *) -> Prop :=
+  | AstNil: forall stc ioss soss, AtomicSteps stc ioss soss nil
+  | AstSpecSilent:
+      forall pre pioss soss msg curs1 curs2 curs,
+        R pioss soss ->
+        curs = curs1 ++ msg :: curs2 ->
+
+        (forall pmsg obj ostc stc piost niost nioss,
+            msg_id msg = pmsg_mid pmsg ->
+            In pmsg (obj_trs obj) ->
+            In obj (sys_objs impl) ->
+            StepCondHolds stc (msg_value msg) pioss ->
+            pioss@[obj_idx obj] = Some piost ->
+            (OstCondHolds ostc niost ->
+             pmsg_postcond pmsg niost (msg_value msg) niost) ->
+            nioss = pioss +[obj_idx obj <- niost] ->
+            R nioss soss /\
+            AtomicSteps (updateOstCond (obj_idx obj) ostc stc)
+                        nioss soss
+                        (curs ++ pmsg_outs pmsg piost (msg_value msg))) ->
+
+        AtomicSteps pre pioss soss curs.
+  (* TODO: | AstSpecStep: ... *)
+
+  Definition CompleteAtomicSteps (ioss soss: ObjectStates) (rqin: Msg) :=
+    AtomicSteps stepCondTop ioss soss (rqin :: nil).
+
+  Theorem atomicSteps_trsSimStepAtomic:
+    forall ioss soss,
+      AtomicSteps stepCondTop ioss soss (rqImpl :: nil) ->
+      ioss ≈ soss ->
+      forall ist1 sst1,
+        tst_oss ist1 = ioss ->
+        tst_oss sst1 = soss ->
+        forall ihst ist2 mouts,
+          steps_det impl ist1 ihst ist2 ->
+          Atomic impl trsIdx (toTMsgU rqImpl) ihst mouts ->
+          exists sst2 shst,
+            steps_det spec sst1 shst sst2 /\
+            map p (behaviorOf impl ihst) = behaviorOf spec shst /\
+            tst_oss ist2 ≈ tst_oss sst2.
+  Proof.
+  Admitted.
+
+End AtomicSteps.
+
